\setcounter{chapter}{9}
\chapter{Parametric Equation and Polar Coordinate}
\section{Parametric Equation}
\noindent
\hfill
\begin{minipage}{0.3\textwidth}
$$x=1\Rightarrow y=1$$
$$x=?\Rightarrow y=?$$
$$y=f(x)$$
\end{minipage}
\begin{minipage}{0.3\textwidth}
\includegraphics[width=\linewidth]{1.jpg}
\end{minipage}
\begin{minipage}{0.3\textwidth}
$$y=t+1$$
$$x=1-t^2$$
$$t=1\Rightarrow $$
$$x=0~,y=2,(0,2)$$
\end{minipage}
\noindent{\color{smalt(darkpowderblue)}\rule{\linewidth}{.2mm}}
%-----------------------------------------------------------------------------------
\begin{example}
Sketch the curve define by the \textbf{\color{smalt(darkpowderblue)} Parametric equation}\\
$x=t^2-2t~,~y=t+1.$\\
\underline{\textbf{\large}\color{smalt(darkpowderblue)}Solution} \\
\begin{minipage}{0.25\textwidth}
	\begin{tabular}{ |c | c | c | }
	\hline
	t & x & y \\
{\color{red}2} & {\color{red}0} & {\color{red}3}\\
{\color{red}1} & {\color{red}-1} & {\color{red}2}\\
		0 & 0 & 1\\
{\color{red}-1} & {\color{red}3}& {\color{red}0}\\
{\color{red}-2} & {\color{red}8}& {\color{red}-1}\\
        \vdots &\vdots &\vdots
	\end{tabular}
\end{minipage}
\begin{minipage}{0.35\textwidth}
{\color{smalt(darkpowderblue)}$$t=y-1$$
$$\Downarrow$$
$$x=(y-1)^2-2(y-1)$$
$$=y^2-2y+1-2y+2$$
$$x=y^2-4y+2$$}
\end{minipage}
\begin{minipage}{0.6\textwidth}
\includegraphics[width=5cm]{2.jpg}
\end{minipage}
\end{example}
%----------------------------------------------------------------------------------
\begin{example}
Sketch $x=t^2-2t~,~y=t+1~,~-1\leq x\leq 2.$\\
\underline{\textbf{\large}\color{smalt(darkpowderblue)}Solution} \\
\begin{minipage}{0.6\textwidth}
$${\color{smalt(darkpowderblue)}Parametric~equation:}$$
$$x=f(t)~,~y=g(t)$$
$$a\leq t\leq b$$
$$Initial~point~(f(a),g(a))$$
$$Terminal~point~(f(b),g(b))$$
\end{minipage}
\noindent\begin{minipage}{0.5\textwidth}
\includegraphics[width=5cm]{3.jpg}
\end{minipage}
\hfill
\end{example}
\noindent{\color{smalt(darkpowderblue)}\rule{\linewidth}{.2mm}}
%%%%%%%%%%%%%%%%%%%%%%%%%%%%%%%%%%%%%%%%%%%%%%%%%%%%%%%%%%%%%%%%%%%%%%5
\begin{example}
Sketch $x=\cos t~,~y=\sin t$\\
\underline{\textbf{\large}\color{smalt(darkpowderblue)}Solution}\\
\begin{minipage}{0.5\textwidth}
$$\cos^2 t+\sin^2 t=1$$
$$x^2+y^2=1$$
$$t=0\Rightarrow (1,0)$$
$$t=\cfrac{\pi}{2}\Rightarrow (0,1)$$
\end{minipage}
\begin{minipage}{0.5\textwidth}
\includegraphics[width=5cm]{4.jpg}
\end{minipage}
\end{example}
%------------------------------------------------------------------------
\noindent{\color{smalt(darkpowderblue)}\rule{\linewidth}{.2mm}}
%-------------------------------------------------------------
\begin{example}
Sketch $x=\cos 2t~,~y=\sin 2t$\\
\underline{\textbf{\large}\color{smalt(darkpowderblue)}Solution} \\
\begin{minipage}{0.5\textwidth}
$$\cos^2 2t+\sin^2 2t=1$$
$$x^2+y^2=1$$
$$t=0\Rightarrow (0,0)$$
$$t=\cfrac{\pi}{2}\Rightarrow (-1,0)$$
\end{minipage}
\begin{minipage}{0.5\textwidth}
\includegraphics[width=5cm]{4.jpg}
\end{minipage}
\end{example}
%----------------------------------------------------------------------------------
\begin{exercise}
Sketch $x=\cos\cfrac{1}{2}t~,~y=\sin\cfrac{1}{2}t$ 
\end{exercise}
%----------------------------------------------------------------------------------

\begin{example}
Sketch $x=2\cos t~,~y=2\sin t$\\
\underline{\textbf{\large}\color{smalt(darkpowderblue)}Solution} \\
\begin{minipage}{0.5\textwidth}
$$x^2+y^2=4\cos^2 t+4\sin^2 t$$
$$x^2+y^2=4$$
\end{minipage}
\begin{minipage}{0.5\textwidth}
\includegraphics[width=5cm]{5.jpg}
\end{minipage}
\end{example}
\noindent{\color{smalt(darkpowderblue)}\rule{\linewidth}{.2mm}}

%---------------------------------------------------------------------------------
\begin{example}
Sketch $x=2\cos t+1~,~y=2\sin t+2$\\
\underline{\textbf{\large}\color{smalt(darkpowderblue)}Solution} \\
\begin{minipage}{0.48\textwidth}
$$x=2\cos t+1\Rightarrow x-1=2\cos t$$
$$y=2\sin t+2\Rightarrow y-2=s\sin t$$
$$(x-1)^2+(y-2)^2=4(\cos^2 t+\sin^2 t)$$
$$(x-1)^2+(y-2)^2=4$$
\end{minipage}
\begin{minipage}{0.18\textwidth}
\includegraphics[width=5cm]{6.jpg}
\end{minipage}
\begin{minipage}{0.5\textwidth}
$$x=r\cos t+h$$
$$y=r\sin t+k$$
$$circle~center~(h,k)$$
$$radius~r$$
\end{minipage}
\end{example}

\noindent{\color{smalt(darkpowderblue)}\rule{\linewidth}{.2mm}}
%----------------------------------------------------------------------------------
\begin{example}
Sketch $x=2\cos t~,~y=3\sin t$\\
\underline{\textbf{\large}\color{smalt(darkpowderblue)}Solution}\\
\begin{minipage}{0.5\textwidth}
$$x=2\cos t\Rightarrow \cos t=\cfrac{x}{2}$$
$$y=3\sin t\Rightarrow\sin t=\cfrac{y}{3}$$
$$\Rightarrow (\cfrac{x}{2})^2+(\cfrac{y}{3})^2=1$$
\end{minipage}
\begin{minipage}{0.5\textwidth}
\includegraphics[width=5cm]{5.jpg}
\end{minipage}
\end{example}
%----------------------------------------------------------------------------------
\begin{example}
Sketch $x=\sin t~,~y=\sin^2 t$\\
\underline{\textbf{\large}\color{smalt(darkpowderblue)}Solution} \\
\begin{minipage}{0.5\textwidth}
$$y=x^2$$
$$t=0\Rightarrow(0,0)$$
$$t=\cfrac{\pi}{2}\Rightarrow(1,1)$$
$$t=\pi\Rightarrow(0,0)$$
$$t=\cfrac{3}{2}\pi\Rightarrow(-1,1)$$
$$t=2\pi\Rightarrow(0,0)$$
\end{minipage}
\begin{minipage}{0.5\textwidth}
\includegraphics[width=5cm]{7.jpg}
\end{minipage}
\end{example}
\noindent{\color{smalt(darkpowderblue)}\rule{\linewidth}{.2mm}}
%----------------------------------------------------------------------------------
\begin{example}
$\boxed{\cfrac{37}{628}}$\begin{enumerate}
    \item[(a)] $x=t^3~,~y=t^2$, {\color{red}$\Rightarrow t=x^\frac{1}{3}\Rightarrow y=x^\frac{2}{3}$}
    \item[(b)] $x=t^{6}~,~y=t^{4}$, {\color{red}$t=x^{\frac{1}{6}}\Rightarrow y=x^\frac{4}{6}\Rightarrow y=x^\frac{2}{3}$}
    \item[(c)] $x=e^{-3t}~,~y=e^{-2t}$, {\color{red}$\Rightarrow x=(e^{-t})^3\Rightarrow e^{-t}=x^\frac{1}{3}\Rightarrow y=(e^{-t})^2=(x^\frac{1}{3})^2\Rightarrow y=x^\frac{2}{3}$}
    \end{enumerate}
    \underline{\textbf{\large}\color{smalt(darkpowderblue)}Solution} \\
    \begin{minipage}{0.1\textwidth}
$$(a) ~ x=t^6$$
$$y=t^4$$
$$y=x^\frac{2}{3}$$\\
\end{minipage} 
\begin{minipage}{0.62\textwidth}
$$(b)  x=t^6$$
$$y=t^4$$
$$y=x^\frac{2}{3}$$\\
\end{minipage} 
\begin{minipage}{0.18\textwidth}
$$(c)~x=e^{-3t}=\cfrac{1}{e^{3t}}$$
$$y=e^{-2t}=\cfrac{1}{e^{2t}}$$
$$y=x^\frac{2}{3}$$\\
\end{minipage}\\ 
\noindent\begin{minipage}{0.3\textwidth}
\includegraphics[width=4.2cm]{h1.jpg}
$$t=-1 \Rightarrow (-1,1) $$
$$t=0 \Rightarrow (0,0)$$
$$t=1 \Rightarrow (1,1)$$
\end{minipage}
\noindent\begin{minipage}{0.4\textwidth}
\includegraphics[width=4.2cm]{h2.jpg}
$$t=-1 \Rightarrow (1,1) $$
$$t=0 \Rightarrow (0,0)$$
$$t=1 \Rightarrow (1,1)$$
\end{minipage}
\noindent\begin{minipage}{0.3\textwidth}
\includegraphics[width=4.2cm]{h3.jpg}
$$t=-1 \Rightarrow (e^3,,e^2) $$
$$t=0 \Rightarrow (1,1)$$
$$t=1 \Rightarrow (\cfrac{1}{e^3},\cfrac{1}{e^2})$$
\end{minipage}
\end{example}