
%%%%%%%%%%%%%%%%%%%%%%%%%%%%%%%%%%%%%%%%%%%%%%%%%%%%%%%%%%%%%%%%%%%%-----------------------
\underline{\large\textbf{\color{smalt(darkpowderblue)}{Cycloid}}}
\noindent\begin{minipage}{0.3\textwidth}
\includegraphics[width=4cm]{h5.jpg}
\end{minipage}
\noindent\begin{minipage}{0.3\textwidth}
\includegraphics[width=4cm]{h4.jpg}
\end{minipage}
\noindent\begin{minipage}{0.3\textwidth}
\includegraphics[width=4cm]{h6.jpg}
\end{minipage}\\
\hspace*{1.8cm}$$\underbrace{x=r(\theta-sin\theta)~~y=r(1-cos\theta)}~ ~0 \leq \theta \leq 2*\pi$$
$$Cycloid$$\\
\noindent{\color{smalt(darkpowderblue)}\rule{\linewidth}{.2mm}}
%%%%%%%%%%%%%%%%%%%%%%%%%%%%%%%%%%%%%%%%%%%%%%%%%%%%%%%%%%%%%%%%%%%
\begin{problem}
1, 3, 4, 7, 8, 10, 12, 15, 16, 25, 26, 37.
\end{problem}
%%%%%%%%%%%%%%%%%%%%%%%%%%%%%%%%%%%%%%%%%%%%%%%%%%%%%%%%%%%%%%%%%%%%-
\section{Calculus with Parametric Equations.}
let $x=f(t) , y=g(t)$   Then \\ $$\cfrac{dy}{dx}=\cfrac{\cfrac{d(y)}{d(t)}}{\cfrac{d(x)}{d(t)}}=\cfrac{g'(t)}{f'(t)}\hspace{.5cm} ,f'(t)\neq 0$$
%%%%%%%%%%%%%%%%%%%%%%%%%%%%%%%%%%%%%%%%%%%%%%%%%%%%%%%%%%%%%%%%%%%%
\begin{example}
if $x=cost , y=sint$\hspace{1cm}\\
\underline{\textbf{\large}\color{smalt(darkpowderblue)}Solution} \\
$$\cfrac{dy}{dx}=-\cfrac{cost}{sint}=-cott$$
  \begin{equation}
\begin{split} \cfrac{d^2y}{dx^2} &=\cfrac{d}{dx} \cfrac{dy}{dx} = \cfrac{\cfrac{d}{dt}\cfrac{dy}{dx}}{\cfrac{dx}{dt}} \\
&= \cfrac{csc^2t}{-sint} \\
&= -csc^3t
\end{split}
\end{equation}
\end{example}
%%%%%%%%%%%%%%%%%%%%%%%%%%%%%%%%%%%%%%%%%%%%%%%%%%%%%%%%%%%%%%%%%%%%-
\noindent{\color{smalt(darkpowderblue)}\rule{\linewidth}{.2mm}}
\begin{example}
if $x=t^3 , y=3t$, Find $\cfrac{d^2y}{dx^2}$\\
\underline{\textbf{\large}\color{smalt(darkpowderblue)}Solution} \\
\noindent\begin{minipage}{0.3\textwidth}
$$\cfrac{dy}{dx}=\cfrac{3}{3t^2}=t^{-2}$$
$$\cfrac{d^2y}{dx^2}=\cfrac{\cfrac{d}{dt}\cfrac{dy}{dx}}{\cfrac{dx}{dt}}$$ 
$$\cfrac{-2t^{-3}}{3t^2} = \cfrac{-2}{3}t^{-5}$$
$$\cfrac{d^2y}{dx^2}=\cfrac{-2}{3}x^\frac{-5}{3}$$
\end{minipage}
\noindent\begin{minipage}{0.6\textwidth}
$$y=3x^\frac{1}{3}$$
$$\cfrac{dy}{dx}=x^\frac{-2}{3}$$
\color{smalt(darkpowderblue)}{$$\cfrac{d^2y}{dx^2}=\cfrac{-2}{3}x^\frac{-5}{3}$$}
$\swarrow$
\end{minipage}
\end{example}
%%%%%%%%%%%%%%%%%%%%%%%%%%%%%%%%%%%%%%%%%%%%%%%%%%%%%%%%%%%%%%%%%%%%-
\begin{exercise}
if $y=cost+t ,\\ x=1-t+t^2$ \hspace{5mm}~Find $\cfrac{d^2y}{dx^2}$ 
\end{exercise}
%%%%%%%%%%%%%%%%%%%%%%%%%%%%%%%%%%%%%%%%%%%%%%%%%%%%%%%%%%%%%%%%%%%%
\begin{example}
Consider the parametric equations : $x=t^2 , y=t^3-3t$
\begin{enumerate}
    \item[(a)] Show that hte curve has two tangents at (3,0) ,Find the tangent line
    \item[(b)]Find where the tangent is horizontal ? Vertical ?
    \item[(c)]Find where the curve is concave up? down ?
    \item[(d)]Sketch the curve .
\end{enumerate}
\underline{\textbf{\large}\color{smalt(darkpowderblue)}Solution} \\
(a)~$(3,0) \Rightarrow ~x=3 ~, y=0$\\$t^2=3 \hspace{3cm} t^3-3t=0$ $\\ \downarrow \hspace{4cm} \downarrow \\ t=\sqrt{3} , -\sqrt{3} \hspace{2cm} t=0 ,\sqrt{3} , -\sqrt{3} $ \hspace{1cm} {\color{red}Refuse t=0} \\
The curve passes the point (3,0) two times at $t=\sqrt{3} , -\sqrt{3} $ \\ 
$\cfrac{dy}{dx}=\cfrac{\cfrac{dy}{dt}}{\cfrac{dx}{dt}} = \cfrac{3t^-3}{2t}$ \\ 
at $t=\sqrt{3}\Rightarrow \cfrac{dy}{dx}=\cfrac{3\sqrt{3}^2-3}{2\sqrt{3}}=\cfrac{3}{\sqrt{3}}=\sqrt{3}$\\
at $t=-\sqrt{3}\Rightarrow \cfrac{dy}{dx}=\cfrac{3*3-3}{-2\sqrt{3}}=-\sqrt{3}$ \\
So equation (1) \\
$y-0=\sqrt{3}(x-3)$\\
And equation (2) \\
$y-0=-\sqrt{3}(x-3)$\\
\end{example}

\noindent{\color{smalt(darkpowderblue)}\rule{\linewidth}{.2mm}}
