\begin{itemize}
\item $ {\overrightarrow{a}}\times{\overrightarrow{b}} =
\begin{vmatrix}
{i} & {j} & {k} \\
a_{1} & a_{2} & a_{3} \\
b_{1} & b_{2} & b_{3} 
\end{vmatrix}$
\item $a \times {\overrightarrow{b}} \perp {\overrightarrow{a}} \& {\overrightarrow{a}} \times {\overrightarrow{b}} \perp {\overrightarrow{b}}$
\item $\ \mid{\overrightarrow{a}}\times{\overrightarrow{b}}\mid = \mid{\overrightarrow{a}}\mid  \mid{\overrightarrow{b}}\mid sin \theta$ \hspace{2cm} $g \in [0,\pi ]$
\item $ \mid{\overrightarrow{a}}\times{\overrightarrow{b}} =$ area of the parallelogram that determined by ${\overrightarrow{a}}\times{\overrightarrow{b}}$ 
\end{itemize}
\noindent{\color{smalt(darkpowderblue)}\rule{\linewidth}{.2mm}}
%===========================================================
\begin{example}
find the area of the triangle with vertices\\
{\color{smalt(darkpowderblue)}{\underline{Solution}}} :
\begin{itemize}
\item $P(2,1,3)$
\item $Q(1,-1,1)$
\item $R(3,2,-2)$
\item ${\overrightarrow{PQ}} = < -1,-2,-2 > $
\item  ${\overrightarrow{PR}} = < 1,1,-5 >$
\item $A = \mid{\overrightarrow{PQ}}\times{\overrightarrow{PR}}\mid$
\end{itemize}
${\overrightarrow{PQ}}\times{\overrightarrow{PR}}$=
$\begin{vmatrix}
{i} & {j} & {k} \\
{-1} & {-2} & {-2} \\
{1} &{1} & {-5} \\
\end{vmatrix}$
$= <12,-7,1>$\\ \\
$\Rightarrow A =   \mid{\overrightarrow{PQ}}\times{\overrightarrow{PR}}\mid \\ 
=  \sqrt{144+49+1} \\
= \sqrt{194}$ \\
\end{example}
\noindent{\color{smalt(darkpowderblue)}\rule{\linewidth}{.2mm}}
%===================================================================
\begin{example}
Find 
\begin{enumerate}
\item $i \times i$
\item $i \times j $
\item $k \times j$
\item $<-1,-2,-2> \times <1,1,-5> $
\end{enumerate}
{\color{smalt(darkpowderblue)}{\underline{Solution}}} :
\begin{enumerate}
\item $ {\overrightarrow{0}} = <0,0,0>$
\item $ k$
\item $-i$
\item $= (-i -2j -2k) \times (i + j -5k)$\\
$ = -k -5j +2k +10i -2j +2i $\\
$= <12,-7,1>$
\end{enumerate}
\end{example}
\noindent{\color{smalt(darkpowderblue)}\rule{\linewidth}{.2mm}}
%==========================================================
\begin{example}
True or False :
\begin{enumerate}
\item ${\overrightarrow{a}}\times{\overrightarrow{b}} = {\overrightarrow{b}}\times{\overrightarrow{a}}$
\item  $({\overrightarrow{a}}\times{\overrightarrow{b}}) \times {\overrightarrow{c}} = {\overrightarrow{a}}\times ({\overrightarrow{b}}\times \overrightarrow{c}) $
\item  $i\times(i \times j) = i \times k = -j$\\
$(i \times i) \times j = \overrightarrow{0} \times i = \overrightarrow{0}$
\end{enumerate}
{\color{smalt(darkpowderblue)}{\underline{Solution}}} :
\begin{enumerate}
\item False : ~ $ i \times j = k \neq j \times i = -k $
\item False \begin{itemize}
\item $ i\times(i \times j) = i \times k = -j$
\item $(i \times i) \times j = \overrightarrow{0} \times i = \overrightarrow{0}$
\end{itemize}
\end{enumerate}
\end{example}
\noindent{\color{smalt(darkpowderblue)}\rule{\linewidth}{.2mm}}
{\color{smalt(darkpowderblue)}{\underline{Properties}}} : 
\begin{enumerate}
\item  ${\overrightarrow{a}}\times{\overrightarrow{b}} = -{\overrightarrow{b}}\times{\overrightarrow{a}}$
\item $(c{\overrightarrow{a}})\times{\overrightarrow{b}} = {\overrightarrow{a}}\times (c{\overrightarrow{b}}) = c({\overrightarrow{a}}\times{\overrightarrow{b}}) $
\item ${\overrightarrow{a}}\times({\overrightarrow{b}} + \overrightarrow{c}) = {\overrightarrow{a}}\times{\overrightarrow{b}} + {\overrightarrow{a}}\times{\overrightarrow{c}}$
\item $(\overrightarrow{a} + \overrightarrow{b}) \times \overrightarrow{c} = {\overrightarrow{a}}\times{\overrightarrow{c}} + {\overrightarrow{b}}\times{\overrightarrow{c}}$
\item $\overrightarrow{a} \cdot (\overrightarrow{b} \times \overrightarrow{c}) = (\overrightarrow{a} \times \overrightarrow{b}) \cdot \overrightarrow{c}$
\item $\overrightarrow{a} \times (\overrightarrow{b} \times \overrightarrow{c}) = (\overrightarrow{a} \cdot \overrightarrow{c}) \overrightarrow{b} - (\overrightarrow{a} \cdot \overrightarrow{b})\overrightarrow{c}$
\end{enumerate}
{\color{smalt(darkpowderblue)}{Pf(5)}} if :
\begin{itemize}
\item $\overrightarrow{a} = <a_{1} , a_{2} , a_{3} >$
\item $\overrightarrow{b} = < b_{1} , b_{2} , b_{3} >$
\item $\overrightarrow{c} = <c_{1} , c_{2} , c_{3}>$
\end{itemize}
{\color{smalt(darkpowderblue)}{\underline{L.H.S}}}\\ = $\overrightarrow{a} \cdot (\overrightarrow{b} \times \overrightarrow{c})$\\
$= <a_{1},a_{2},a_{3}> \cdot <b_{2}c_{3} - b_{3}c_{2} , b_{3}c_{1} - b_{1}c_{3} , b_{1}c_{2} -b_{2}c_{1} >$\\
$= a_{1}b_{2}c_{3} - a_{1}b_{3}c_{2} + a_{2}b_{3}c_{1} - a_{2}b_{1}c_{3} + a_{3}b_{1}c_{2} - a_{3}b_{2}c_{1}$\\
{\color{smalt(darkpowderblue)}{\underline{R.H.S}}}\\ = $(\overrightarrow{a} \times \overrightarrow{b}) \cdot \overrightarrow{c}$\\
$= <a_{2}b_{3} - a_{3}b_{2} , a_{3}b_{1} - a_{1}b_{3} , a_{1}b_{2} - a_{2}b_{2} > \cdot <c_{1} , c_{2}, c_{3} >\\
= a_{2}b_{3}c_{1} - a_{3}b_{2}c_{1} + a_{3}b_{1}c_{2} - a_{1}b_{3}c{2} + a_{1}b_{2}c_{3} + a_{2}b_{1}c_{3}\\
\Rightarrow$ {\color{smalt(darkpowderblue)}{L.H.S }}={\color{smalt(darkpowderblue)}{ R.H.S}} \\
\noindent{\color{smalt(darkpowderblue)}\rule{\linewidth}{.2mm}}
\begin{example}
If  $\overrightarrow{a}\cdot(\overrightarrow{b} \times \overrightarrow{c}) = 2$ ,\\ Find $2 \overrightarrow {b} \cdot (\overrightarrow{a} \times 2 \overrightarrow{c})$\\
{\color{smalt(darkpowderblue)}{\underline{Solution}}} : \\
$ = 4 \overrightarrow{b} \cdot (\overrightarrow{a} \times \overrightarrow{c})\\
= 4 (\overrightarrow{a} \times \overrightarrow{c}) \cdot \overrightarrow{b}\\
= 4 \overrightarrow{a} \cdot (\overrightarrow{c} \times \overrightarrow{b})\\
= -4 \overrightarrow{a} \cdot (\overrightarrow{b} \times \overrightarrow{c})\\ =-8$\end{example}
\noindent{\color{smalt(darkpowderblue)}\rule{\linewidth}{.2mm}}