{{\color{smalt(darkpowderblue)}{\underline{Plane}}}}
\begin{itemize}
    \item $ p(x_0 , y_0 , z_0)$
    \item $\overrightarrow{n} = <a,b,c>$\\
$ax+by+cz+d = 0$\\
$d=-(ax_\cdot + by_\cdot +cz_\cdot)$
\end{itemize}
\noindent{\color{smalt(darkpowderblue)}\rule{\linewidth}{.2mm}}
\begin{example}
Find the equation of the plane that passes through the point 
p(1,2,1), Q(2,3,2), R(-1,-1,3)\\
{{\color{smalt(darkpowderblue)}{\underline{Solution}}}} \\
$ax+by+cz+d=0 $ 
\begin{itemize}
    \item if $d\neq 0 $ \\ $Ax+By+Cz+1=0 \\ 
    A+2B+C+1=0 \\ 2A+3B+2C+1=0 \\ -A-B-3C+1=0 $ \hspace{1cm} (Rejected)
    \item $d=0 \\ ax+by+cz+1=0$
\end{itemize}
\end{example}
\noindent{\color{smalt(darkpowderblue)}\rule{\linewidth}{.2mm}}
\begin{example}
Find the equation of the plane that passes through the point (1,-1,2) \& contains the line \\
$L_{1} : \cfrac{x-1}{2} = \cfrac{y+1}{2} = \cfrac{z-1}{3}. \overrightarrow{\nu} = <2,3,1>$\\
{{\color{smalt(darkpowderblue)}{\underline{Solution}}}}
\begin{enumerate}
    \item  Point $(1,-1,2)$
    \item  normal vector 
    \begin{align*}
&\overrightarrow{n} = \overrightarrow{r} \times \overrightarrow{\nu}\\
&=\overrightarrow{RQ} \times \overrightarrow{\nu}\\
&=<0,0,1> \times <2,2,3>\\
&-2x+2y+0z+4=0\\
&\Rightarrow x-y-2=0
\end{align*}
\end{enumerate}
\end{example} 
\noindent{\color{smalt(darkpowderblue)}\rule{\linewidth}{.2mm}}
\begin{example}
find the equations of the line of intersection of the following planes .\\
$P_{1} : 2x-y+z_3 = 0 . \overrightarrow{n_{1}} = <2,-1,1>$\\
$P_{2} : x-3y-z-1=0 . \overrightarrow{n_{2}}=<1,-3,-1>$\\
{{\color{smalt(darkpowderblue)}{\underline{Solution}}}}
\begin{itemize}
    \item Point :$ P(0,-1,2) $
    \item Parallel vector \\ 
    $\overrightarrow{\nu} = \overrightarrow{n_{1}} \times \overrightarrow{n_{2}}$
=$\begin{vmatrix}
 {i} & {j} & {k} \\
  2 & -1 & 1 \\
  1 & -3 & -1 
 \end{vmatrix}$\\
 $=<4,3,-5>$ 
 let x=0 \\ 
 $-y +z=3$\\
 +\\
 $-3y-z=1$\\
 $\Rightarrow -4y = 4 \Rightarrow y =-1 \\ \Rightarrow z=2$\\
 $x=0+4t$\\
 $y=-1+3t$\\
 $z=2-5t$\\
\end{itemize} 
\noindent{\color{smalt(darkpowderblue)}\rule{\linewidth}{.2mm}}
{{\color{smalt(darkpowderblue)}{\underline{Solution 2}}}} : Pick two points on the line :
 \begin{itemize}
     \item  $P(0,-1,2) $
     \item $Q(\cfrac{4}{3},0,\cfrac{1}{3})$
 \end{itemize}
  Let $y=0$  
  $$2x+z=3 $$
$$+$$
$$x-z=1 $$
$$\Rightarrow 3x=4$$  $$\Rightarrow x=\cfrac{4}{3}$$
$$\Rightarrow z=\cfrac{4}{3} -1 = \cfrac{1}{3}$$
$\overrightarrow{\nu} = \overrightarrow{PQ} = <\cfrac{4}{3},1,\cfrac{-5}{3}>$
\begin{itemize}
    \item $x=0+\cfrac{4}{3} t$
    \item $y=-1+t$
    \item $z=2-\cfrac{5}{3} t$
\end{itemize}
\noindent{\color{smalt(darkpowderblue)}\rule{\linewidth}{.2mm}}
{{\color{smalt(darkpowderblue)}{\underline{Solution 3 }}}}: \\
$2x-y+z-3 =0$\\   
$x-3y-z-1=0$\\   let $x=t $\\ 
$\Rightarrow 2t-y+z-3 = 0$ \\
$\Rightarrow t-3y-z-1=0$\\
$\downarrow$\\
$-y+z=3-2t$\\
+\\
$-3y-z=1-t$\\ \\
$\Rightarrow -4y = 4-3t\\ \Rightarrow y=-1+\cfrac{3}{4} t$\\
$-3(-1+\cfrac{3}{4}t) -z = 1-t$\\
$z=3-\cfrac{9}{4}t - 1+t$\\
$z=2-\cfrac{5}{4} t$
\end{example} 
\begin{remark}
  \begin{itemize}
      \item  two plane are parallel if their normal vectors are parallel .
      \item  the angle blw too plane is defined to be the  active angle blw $\overrightarrow{n_{1}} \& \overrightarrow{n_{2}}.$
  \end{itemize}
\end{remark}
%===================================================================
\begin{example}
find the angle btw the following plane : 
$ 2x-2y=z-1 = 0 \\
x=3y-z=7 = 0 ,.$
{{\color{smalt(darkpowderblue)}{\underline{Solution}}}}: 
\begin{itemize}
    \item $ \overrightarrow{n_{1}} = <2,-2,1>$
    \item $\overrightarrow{n_{2}} = <1,3,-1>$
\end{itemize}
$\theta : cos\theta = \cfrac{\overrightarrow{n_1} \cdot \overrightarrow{n_2}}{\mid \overrightarrow{n_1}\mid \mid \overrightarrow{n_2}\mid} = \cfrac{2-6-1}{3\sqrt{11}} = -\cfrac{5}{3\sqrt{11}} \approx 120.1\\
\Rightarrow \alpha = 59.9$\end{example}
\noindent{\color{smalt(darkpowderblue)}\rule{\linewidth}{.2mm}}
\begin{example}
 find the intersection btw the following line :\\
$P:2x-2y+z_1 = 0 $\\
$L: x=1+t , y=1-t , z=t .$\\
{{\color{smalt(darkpowderblue)}{\underline{Solution}}}}:\\ 
 $2(1+t) -2(1-t) +t-1 = 0$\\
$2+2t-2+2t+t=1$\\
$5t = 1\Rightarrow t=\cfrac{1}{5}$\\
$x=1+\cfrac{1}{5} \Rightarrow \cfrac{6}{5}$\\
$y=1-\cfrac{1}{5} \Rightarrow \cfrac{4}{5}$\\
$z=\cfrac{1}{5}$
\end{example}
\noindent{\color{smalt(darkpowderblue)}\rule{\linewidth}{.2mm}}