\noindent{\color{smalt(darkpowderblue)}\rule{\linewidth}{.2mm}}
{\color{smalt(darkpowderblue)}{Partial differential Equation:}}
\begin{enumerate}
    \item Laplace's Equation:
    $\cfrac{\partial^2 u}{\partial x^2}+\cfrac{\partial^2 u}{\partial y^2}=0$\\
    Solution of this equation are called :{\color{smalt(darkpowderblue)}harmonic equation}\\

    \begin{example}
    show that $u(x,y)=x^2-y^2$ is harmonic \\
    $u_x=2x$ , $u_y=-2y$\\
    $u_{xx}=2$, $u_{yy}=-2$\\
    so $u_{xx}+u_{yy}=0$
    \end{example}
    \noindent{\color{smalt(darkpowderblue)}\rule{\linewidth}{.2mm}}

    \begin{example}
    show that $u(x,y)=e^x\cos{y}$ satisfies Laplace's equation \\
    $u_x=e^x\sin{y}$ , $u_y=e^x\cos{y}$\\
    $u_{xx}=e^x\sin{y}$ , $u_{yy}=-e^x\sin{y}$\\
    $\Rightarrow u_{xx}+u_{yy}=0$
    \end{example}
    \noindent{\color{smalt(darkpowderblue)}\rule{\linewidth}{.2mm}}

    \item Wave equation \\
       \noindent\begin{minipage}{0.5\textwidth}
    $\cfrac{\partial^2 u}{\partial t^2}=a^2\cfrac{\partial^2 u}{\partial x^2}$\\
\end{minipage}
    \noindent\begin{minipage}{0.5\textwidth}
\begin{center}
   \includegraphics[width=6cm]{ss1.png}\\
\end{center}\end{minipage}
\end{enumerate}
    \begin{example}
    show that $u(x,t)=\sin{x-at}$ satisfies the wave equation \\
    $u_t=-acos(x-at)$ , $u_x=cos(x-at)$\\
    L.H.S=$u_{tt}=-a^2sin(x-at)$ , R.H.S=$u_{xx}=-sin(x-at)$\\
    L.H.S=R.H.S
    \end{example}
\noindent{\color{smalt(darkpowderblue)}\rule{\linewidth}{.2mm}}
\begin{problem}
5,7,8,9,12,13,14,1821,25,29,31,33,37,39,40
\end{problem}
\section{Tangent Plane and Linear Approximation}
Let $z=f(x,y)$ then the tangent plane at $(x_\circ,y_\circ)$\\
$z=z_\circ=f_x(x_\circ,y_\circ)(x-x_\circ)+f_y(x_\circ,y_\circ)(y-y_\circ)$\\
\noindent{\color{smalt(darkpowderblue)}\rule{\linewidth}{.2mm}}

\begin{example}
Find the tangent plane of $f(x,y)=2x^2+y^2$\\
at $(1,1,3)$\\
$f_x=4x\Rightarrow f_x(1,1)=4$\\
$f_y=2y\Rightarrow f_y(1,1)=2$\\
$z-3=4(x-1)+2(y-1)$\\
$4x+2y-z-3=0$
\end{example}
\noindent{\color{smalt(darkpowderblue)}\rule{\linewidth}{.2mm}}
Linear Approximation: let $z=f(x,y)$, $fx,fy$ cont\\
The linear approximation of $f$ at $(a,b)$\\
is $L(x,y)=f(a,b)+f_x(a,b)(x-a)+f_y(a,b)(y-b)$\\
\noindent{\color{smalt(darkpowderblue)}\rule{\linewidth}{.2mm}}

\begin{example}
let $f(x,y)=x e^{x y}$
\begin{enumerate}
    \item Find linear approximation at $(1,0)$ 
    \item Approximation $f(1.1,-0.1)$\\
\end{enumerate}
{\color{smalt(darkpowderblue)}\underline{Solution:}}\\
$f(1,0)=1$\\
$f_x=xye^{xy}$\\
$f_x(1,0)=1$\\
$f_y=x^2e^{xy}$\\
$f_y(1,0)=1$\\
$\Rightarrow L(x,y)=1+1(x-1)+1(y-0)$\\
$L(x,y)=x+y\approx xe^{xy}$ around $(1,0)$\\
$f(1.1,-0.1)\approx L(1.1,-0.1)=1.1-0.1=1$\\
$f(1.1,-0.1)=0.9854$
\end{example}
\noindent{\color{smalt(darkpowderblue)}\rule{\linewidth}{.2mm}}

\begin{example}
if the tangent plane to $z=f(x,y)$ at $(2,3)$\\
is $2x-3y+z=1\Rightarrow L(x,y)=1-2x+3y$\\
Approximation $f(2.1,2.9)$\\
sol $f(2.1,2.9)\approx 1-2(2.1)+3(2.9)=1-4.2+8.7=5.5$
\end{example}
\noindent{\color{smalt(darkpowderblue)}\rule{\linewidth}{.2mm}}

\begin{example}
Approximation $12\sqrt{8.9}-12\sqrt[3]{8.1}$\\
{\color{smalt(darkpowderblue)}\underline{Solution:}}\\
$f(x,y)=12\sqrt{x}-12\sqrt[3]{y}$ at $(9,8)$\\
$L(x,y)=12+2(x-9)-1(y-8)$\\
$f(8.9,8.1)\approx L(8.9,8.1)=12+2(\cfrac{-1}{10}+\cfrac{-1}{10}$\\
$12-\cfrac{3}{10}=11.7$
\end{example}